\clarification{Polynomial-growth condition implies asymptotic nonnegativity, not asymptotic positivity.}
Since $f(n)$ satisfies the polynomial-growth condition, there exist constants $\widehat{n}>0$ and $d>1$ such that $f(n)/d\le df(n)$ for all $n\ge\widehat{n}$.
Then,
\begin{align*}
    0 &\le df(n)-f(n)/d \\
    &= f(n)(d-1/d) \\
    &= f(n)(d^2-1)/d.
\end{align*}
Because $d>1$, $d^2-1>0$, and $(d^2-1)/d>0$, so the above inequality holds as long as $f(n)\ge0$.
This means that $f(n)$ is asymptotically nonnegative.
