Let $n_0>0$ be the implicit threshold constant, and let $d>0$ be another constant such that $T(n)\le d$ for all $n<n_0$.
We'll prove by induction that
\[
    \lg(n!)-\lg(n_0!) < T(n) \le \lg(n!)+d
\]
for all $n>0$.

Let $0<n<n_0$.
It follows that $0\le\lg(n!)<\lg(n_0!)$, and thus $\lg(n!)-\lg(n_0!)<0\le T(n)\le d\le\lg(n!)+d$.

For the inductive case let $n\ge n_0$ and suppose that
\[
    \lg((n-1)!)-\lg(n_0!) < T(n-1) \le \lg((n-1)!)+d.
\]
We have
\begin{align*}
    T(n) &= T(n-1)+\lg n \\
    &> \lg((n-1)!)-\lg(n_0!)+\lg n \\
    &= \lg((n-1)!\cdot n)-\lg(n_0!) \\
    &= \lg(n!)-\lg(n_0!)
\end{align*}
and
\begin{align*}
    T(n) &= T(n-1)+\lg n \\
    &\le \lg((n-1)!)+d+\lg n \\
    &= \lg((n-1)!\cdot n)+d \\
    &= \lg(n!)+d,
\end{align*}
thereby completing the inductive proof.

By the bounds shown above and by equation (3.28), we obtain $T(n)=\Theta(\lg(n!))=\Theta(n\lg n)$.
