The elements of a Monge array $A$ satisfy the inequality
\[
    A[i,j]+A[k,l] \le A[i,l]+A[k,j],
\]
where $1\le i<k\le m$ and $1\le j<l\le n$.
In particular, it can be $k=i+1$ and $l=j+1$, and thus the ``only if'' part holds.

Now suppose that
\begin{equation} \label{eq:monge-condition-local}
    A[i,j]+A[i+1,j+1] \le A[i,j+1]+A[i+1,j]
\end{equation}
for all $i=1$, 2, \dots, $m-1$ and all $j=1$, 2, \dots, $n-1$.
Fix $i$ and $j$, and let $r\ge0$.
We'll show by induction on $r$ that
\begin{equation} \label{eq:monge-condition-consecutive-columns}
    A[i,j]+A[i+r,j+1] \le A[i,j+1]+A[i+r,j].
\end{equation}
When $r=0$, the inequality holds trivially, establishing the base case.
Now let $r\ge1$ and suppose that \eqref{eq:monge-condition-consecutive-columns} holds for $r-1$.
By the inductive hypothesis and by \eqref{eq:monge-condition-local}, we have
\begin{align*}
    A[i,j]+A[i+r,j+1] &\le A[i,j+1]+A[i+r-1,j]-A[i+r-1,j+1] \\
    &\quad {}+A[i+r-1,j+1]+A[i+r,j]-A[i+r-1,j] \\
    &= A[i,j+1]+A[i+r,j].
\end{align*}

Next we induct on $l$ to show that
\begin{equation} \label{eq:monge-condition}
    A[i,j]+A[k,l] \le A[i,l]+A[k,j]
\end{equation}
holds for all $i$, $j$, $k$, and $l$ such that $1\le i<k\le m$ and $1\le j<l\le n$.
Let's fix $i$, $j$, and $k$.
When $l=j+1$ the inequality reduces to \eqref{eq:monge-condition-consecutive-columns} for $r=k-i$, so let $l>j+1$.
Suppose that \eqref{eq:monge-condition} holds for $l-1$.
Then we have
\begin{align*}
    A[i,j]+A[k,l] &\le (A[i,l-1]+A[k,j]-A[k,l-1])+A[k,l] \\
    &\le (A[i,l-1]+A[k,j]-A[k,l-1]) \\
    &\quad {}+(A[k-1,l]+A[k,l-1]-A[k-1,l-1]) && \text{(by (1))} \\
    &= (A[i,l-1]+A[k-1,l])+A[k,j]-A[k-1,l-1] \\
    &\le A[i,l]+A[k-1,l-1]+A[k,j]-A[k-1,l-1] && \text{(by (2))} \\
    &= A[i,l]+A[k,j].
\end{align*}
